lib/DMFree.fst
@@ -4,7 +4,7 @@ open FStar.Classical.Sugar
 open FStar.List.Tot.Base
 open FStar.Tactics
 
-open Free
+open FFree
 include Hist
 
 (** cmd_wp maps each command to a hist-based WP over events.
@@ -27,7 +27,7 @@ let cmd_wp_sum
     NB: the separate val is needed for extraction: without it, the
     refinements of dm/gdm (where theta appears applied to the two extra
     hist arguments) trip the substitution bug of FStarLang/FStar#490. **)
-val theta : #a:Type u#a -> #cmd:(Type u#0 -> Type u#e) -> #event:Type -> cwp:cmd_wp cmd event -> m:free cmd a -> hist #event a
+val theta : #a:Type u#a -> #cmd:(Type u#0 -> Type u#e) -> #event:Type -> cwp:cmd_wp cmd event -> m:ffree cmd a -> hist #event a
 let rec theta #a #cmd #event cwp m =
   match m with
   | Return x -> hist_return x
@@ -35,7 +35,7 @@ let rec theta #a #cmd #event cwp m =
       hist_bind (cwp op) (fun ri -> theta cwp (k ri))
 
 let lemma_theta_is_monad_morphism_ret #cmd (#event:Type) (cwp:cmd_wp cmd event) (v:'a) :
-  Lemma (theta cwp (free_return #cmd v) == hist_return v) by (compute ()) = ()
+  Lemma (theta cwp (ffree_return #cmd v) == hist_return v) by (compute ()) = ()
 
 let another_lemma (wp1:hist 'a) (wp2:'a -> hist 'b) (wp3:'a -> hist 'b) p h :
   Lemma
@@ -49,9 +49,9 @@ let another_lemma' (wp1:hist 'a) (wp2:'a -> hist 'b) (wp3:'a -> hist 'b) :
 
 private let hist_ord wp1 wp2 = wp2 ⊑ wp1
 
-let rec lemma_theta_is_lax_morphism_bind #a #b #cmd (#event:Type) (cwp:cmd_wp cmd event) (m:free cmd a) (f:a -> free cmd b) :
+let rec lemma_theta_is_lax_morphism_bind #a #b #cmd (#event:Type) (cwp:cmd_wp cmd event) (m:ffree cmd a) (f:a -> ffree cmd b) :
   Lemma
-    (theta cwp (free_bind m f) ⊑ hist_bind (theta cwp m) (fun x -> theta cwp (f x))) =
+    (theta cwp (ffree_bind m f) ⊑ hist_bind (theta cwp m) (fun x -> theta cwp (f x))) =
   match m with
   | Return x ->
     calc (hist_ord) {
@@ -65,10 +65,10 @@ let rec lemma_theta_is_lax_morphism_bind #a #b #cmd (#event:Type) (cwp:cmd_wp cm
       hist_bind (hist_return x) (fun x -> theta cwp (f x));
       `hist_ord` {} (** here there is an eta that forces us to use `hist_ord` **)
       theta cwp (f x);
-      == {} // unfold free_bind
-      theta cwp (free_bind (Return x) f);
+      == {} // unfold ffree_bind
+      theta cwp (ffree_bind (Return x) f);
       == {}
-      theta cwp (free_bind m f);
+      theta cwp (ffree_bind m f);
     }
   | Call op k ->
     calc (hist_ord) {
@@ -84,28 +84,28 @@ let rec lemma_theta_is_lax_morphism_bind #a #b #cmd (#event:Type) (cwp:cmd_wp cm
       hist_bind (cwp op) (fun ri -> hist_bind (theta cwp (k ri)) (fun x -> theta cwp (f x)));
       `hist_ord` {
         let rhs1 = fun ri -> hist_bind (theta cwp (k ri)) (fun x -> theta cwp (f x)) in
-        let rhs2 = fun ri -> theta cwp (free_bind (k ri) f) in
+        let rhs2 = fun ri -> theta cwp (ffree_bind (k ri) f) in
         introduce forall ri. (rhs1 ri) `hist_ord` (rhs2 ri) with begin
           lemma_theta_is_lax_morphism_bind cwp (k ri) f
         end;
         another_lemma' (cwp op) rhs1 rhs2;
         assert (hist_bind (cwp op) rhs1 `hist_ord` hist_bind (cwp op) rhs2) by (assumption ())
       }
-      hist_bind (cwp op) (fun ri -> theta cwp (free_bind (k ri) f));
+      hist_bind (cwp op) (fun ri -> theta cwp (ffree_bind (k ri) f));
       == { _ by (compute ()) } // unfold theta
-      theta cwp (Call op (fun ri -> free_bind (k ri) f));
-      `hist_ord` { _ by (compute ()) } // unfold free_bind
-      theta cwp (free_bind (Call op k) f);
+      theta cwp (Call op (fun ri -> ffree_bind (k ri) f));
+      `hist_ord` { _ by (compute ()) } // unfold ffree_bind
+      theta cwp (ffree_bind (Call op k) f);
       == {}
-      theta cwp (free_bind m f);
+      theta cwp (ffree_bind m f);
     }
 
 // The Dijkstra Monad
 type dm (cmd:Type0 -> Type) (event:Type) (cwp:cmd_wp cmd event) (a:Type) (wp:hist #event a) =
-  (m:(free cmd a){theta cwp m ⊑ wp})
+  (m:(ffree cmd a){theta cwp m ⊑ wp})
 
 let dm_return #cmd (#event:Type) (cwp:cmd_wp cmd event) #a (x : a) : dm cmd event cwp a (hist_return #a #event x) =
-  free_return x
+  ffree_return x
 
 let dm_cmd #cmd (#event:Type) (cwp:cmd_wp cmd event) #r (op:cmd r) :
   dm cmd event cwp r (hist_bind (cwp op) (fun ri -> hist_return ri)) =
@@ -121,7 +121,7 @@ let dm_bind
   (f : (x:a -> dm cmd event cwp b (wp_f x))) :
   Tot (dm cmd event cwp b (hist_bind wp_v wp_f)) =
   lemma_theta_is_lax_morphism_bind cwp v f;
-  free_bind v f
+  ffree_bind v f
 #pop-options
 
 let dm_subcomp #cmd (#event:Type) (cwp:cmd_wp cmd event) #a (wp1 wp2: hist #event a) (f : dm cmd event cwp a wp1) :
